\documentclass{article}
\usepackage[utf8]{inputenc}
\usepackage[italian]{babel}
\usepackage{amsmath}
\usepackage{amsfonts}
\usepackage{amssymb}
\usepackage{xfrac}
\newcommand*{\qed}{\blacksquare}
\newcommand*{\oo}{\infty}
\newcommand*{\limit}[2]{\lim_{#1\rightarrow#2}}
\title{Geometria - Esercizio 4.24}
\author{Riccardo Bergamaschi}
\date{19/10/2023}
\begin{document}
%\maketitle
\[\begin{aligned}
    \sum_{k=0}^{+\oo}\frac{k}{3^k}
    &= \limit{n}{+\oo}\sum_{k=0}^{n}\frac{k}{3^k}\\
    &= \limit{n}{+\oo}\left(\frac{0}{3^0} + \sum_{k=1}^{n}\frac{k}{3^k}\right)\\
    &= \limit{n}{+\oo}\sum_{k=1}^{n}\frac{k}{3^k}\\
    &\ge \limit{n}{+\oo}\sum_{k=1}^{n}\frac{1}{3^k}\\
    &= \limit{n}{+\oo}\left(-1 +\frac{1}{3^0} + \sum_{k=1}^{n}\frac{1}{3^k}\right)\\
    &= \limit{n}{+\oo}\left(-1+\sum_{k=0}^{n}\frac{1}{3^k}\right)\\
    &= \limit{n}{+\oo}\left(-1+\frac{1-\left(\frac{1}{3}\right)^{n+1}}{1-\frac{1}{3}}\right)\\
    &= \limit{n}{+\oo}\left(-1+\frac{3}{2}\left(1-\left(\frac{1}{3}\right)^{n+1}\right)\right)\\
    &= \limit{n}{+\oo}\left(-1+\frac{3}{2}-\frac{3}{2}\left(\frac{1}{3}\right)^{n+1}\right)\\
    &= \limit{n}{+\oo}\left(\frac{1}{2}-\frac{1}{2}\left(\frac{1}{3}\right)^n\right)\\
    &= \frac{1}{2}\limit{n}{+\oo}\left(1-\left(\frac{1}{3}\right)^n\right)\\
    &= \frac{1}{2}\left(1-0\right)\\
    &= \frac{1}{2}\\
\end{aligned}\]
\pagebreak
\[\begin{aligned}
    \sum_{k=0}^{n}\frac{k}{3^k}
    &= \sum_{k=1}^{n}\frac{k}{3^k} \\
    &= \sum_{k=1}^{n}\frac{k-1+1}{3^k} \\
    &= \sum_{k=1}^{n}\frac{k-1}{3^k} + \sum_{k=1}^{n}\frac{1}{3^k} \\
\end{aligned}\]


Ma:


\[\begin{aligned}
    \sum_{k=1}^{n}\frac{k-1}{3^k}
    &= \sum_{k=0}^{n-1}\frac{k}{3^{k+1}} \\
    &= \frac{1}{3}\sum_{k=0}^{n-1}\frac{k}{3^k} \\
    &= \frac{1}{3}\left(\sum_{k=0}^{n}\frac{k}{3^k} - \frac{n}{3^n}\right) \\
    &= \frac{1}{3}\sum_{k=0}^{n}\frac{k}{3^k} - \frac{n}{3^{n+1}} \\
\end{aligned}\]


Allora:


\[\begin{aligned}
    \sum_{k=0}^{n}\frac{k}{3^k}
    &= \sum_{k=1}^{n}\frac{k-1}{3^k} + \sum_{k=1}^{n}\frac{1}{3^k} \\
    &= \frac{1}{3}\sum_{k=0}^{n}\frac{k}{3^k} - \frac{n}{3^{n+1}} + \sum_{k=1}^{n}\frac{1}{3^k} \\
\end{aligned}\]

Ovvero:

\[\begin{aligned}
    \sum_{k=0}^{n}\frac{k}{3^k}
    &= \frac{1}{3}\sum_{k=0}^{n}\frac{k}{3^k} - \frac{n}{3^{n+1}} + \sum_{k=1}^{n}\frac{1}{3^k} \\
    - \frac{1}{3}\sum_{k=0}^{n}\frac{k}{3^k} + \sum_{k=0}^{n}\frac{k}{3^k}
    &= \sum_{k=1}^{n}\frac{1}{3^k} - \frac{n}{3^{n+1}} \\
    \frac{2}{3}\sum_{k=0}^{n}\frac{k}{3^k}
    &= \sum_{k=1}^{n}\frac{1}{3^k} - \frac{n}{3^{n+1}} \\
    \sum_{k=0}^{n}\frac{k}{3^k}
    &= \frac{3}{2}\sum_{k=1}^{n}\frac{1}{3^k} - \frac{n}{2\cdot3^{n}} \\
    &= \frac{3}{2}\left(\sum_{k=0}^{n}\frac{1}{3^k} - 1\right) - \frac{n}{2\cdot3^{n}} \\
    &= \frac{3}{2}\sum_{k=0}^{n}\frac{1}{3^k} - \frac{3}{2} - \frac{n}{2\cdot3^{n}} \\
    &= \frac{3}{2}\cdot\frac{1-\left(\frac{1}{3}\right)^{n+1}}{1-\frac{1}{3}} - \frac{3}{2} - \frac{n}{2\cdot3^{n}} \\
    &= \frac{9}{4}\left(1-\left(\frac{1}{3}\right)^{n+1}\right) - \frac{3}{2} - \frac{n}{2\cdot3^{n}} \\
    &= \frac{9}{4} - \frac{3}{2} - \frac{9}{4\cdot3^{n+1}} - \frac{n}{2\cdot3^{n}} \\
    &= \frac{9-6}{4} - \frac{3}{4\cdot3^n} - \frac{n}{2\cdot3^n} \\
    &= \frac{3}{4} - \frac{2n+3}{4\cdot3^n} \\
\end{aligned}\]

Passando al limite:

\[\begin{aligned}
    \limit{n}{+\oo}\sum_{k=0}^{n}\frac{k}{3^k}
    = \limit{n}{+\oo}\left(\frac{3}{4} - \frac{2n+3}{4\cdot3^n}\right)
    = \frac{3}{4} - 0
    = \frac{3}{4}
\end{aligned}\]

\pagebreak
Fissiamo $\alpha\in\mathbb{R}\setminus\left\{1\right\}$.

\[\begin{aligned}
S &= \sum_{k=0}^n \alpha^k \\
\alpha S &= \sum_{k=0}^n \alpha^{k+1}\\
    &= \sum_{k=1}^{n+1} \alpha^k\\
    &= \sum_{k=1}^{n}\alpha^k + \alpha^{n+1}\\
    &= \sum_{k=0}^{n}\alpha^k + \alpha^{n+1} - \alpha^0\\
    &= S + \alpha^{n+1} - \alpha^0 \\
\alpha S - S &= \alpha^{n+1} - 1 \\
\left(\alpha - 1\right)S &= \alpha^{n+1} - 1 \\
S &= \frac{\alpha^{n+1} - 1}{\alpha - 1} \\
S &= \frac{1 - \alpha^{n+1}}{1 - \alpha} \\
\sum_{k=0}^n \alpha^k &= \frac{1 - \alpha^{n+1}}{1 - \alpha} \\
\end{aligned}\]

\end{document}